\section{(3.3)}

First we assume that $\braket{h|\hat{Q}|h} = \braket{h|\hat{Q}^{\dagger}|h}$ (i.e. $\hat{Q}$ is Hermitian). This doesn't actually say much about the function $h(x)$, since are are already assuming it is in Hilbert space. But the stronger condition that operators must satisfy is that $\braket{f|\hat{Q}|g} = \braket{f|\hat{Q}^{\dagger}|g}$ for any \textit{two} functions $f(x)$ and $g(x)$. To show this, let's first consider the case where $h(x) = f(x) + g(x)$:

\begin{align*}
    \braket{f+g|\hat{Q}|f+g} &= \int(f^* + g^*)[\hat{Q}(f + g)]\;\ddx \\
    &= \int[f^*(\hat{Q}g) + g^*(\hat{Q}g) + f^*(\hat{Q}g) + g^*(\hat{Q}f)]\;\ddx.
\end{align*}

Similarly,

\begin{align*}
    \braket{f+g|\hat{Q}^{\dagger}|f+g} &= \int[\hat{Q}(f^* + g^*)](f + g)\;\ddx \\
    &= \int[(\hat{Q}f^*)f + (\hat{Q}g^*)g + (\hat{Q}f^*)g + (\hat{Q}g^*)f]\;\ddx.
\end{align*}

Since we started with $\braket{h|\hat{Q}|h} = \braket{h|\hat{Q}^{\dagger}|h}$, these two equations must be equal, or better, their integrands must be equal

\begin{equation*}
    f^*(\hat{Q}f) + g^*(\hat{Q}g) + f^*(\hat{Q}g) + g^*(\hat{Q}f) = (\hat{Q}f^*)f + (\hat{Q}g^*)g + (\hat{Q}f^*)g + (\hat{Q}g^*)f.
\end{equation*}

But we can eliminate the first two terms on each side since they are equal by our assumption, so we have

\begin{equation*}
    f^*(\hat{Q}g) + g^*(\hat{Q}f) = (\hat{Q}f^*)g + (\hat{Q}g^*)f.
\end{equation*}

If we now let $h(x) = f(x) + ig(x)$,

\begin{align*}
    \braket{f+ig|\hat{Q}|f+ig} &= \int(f^* - ig^*)[\hat{Q}(f + ig)]\;\ddx \\
    &= \int[f^*(\hat{Q}g) + g^*(\hat{Q}g) + if^*(\hat{Q}g) - ig^*(\hat{Q}f)]\;\ddx,
\end{align*}

and

\begin{align*}
    \braket{f+ig|\hat{Q}^{\dagger}|f+ig} &= \int[\hat{Q}(f^* - ig^*)](f + ig)\;\ddx \\
    &= \int[(\hat{Q}f^*)f + (\hat{Q}g^*)g + i(\hat{Q}f^*)g - i(\hat{Q}g^*)f]\;\ddx.
\end{align*}

Again, these must be equal:

\begin{equation*}
    f^*(\hat{Q}g) + g^*(\hat{Q}g) + if^*(\hat{Q}g) - ig^*(\hat{Q}f) = (\hat{Q}f^*)f + (\hat{Q}g^*)g + i(\hat{Q}f^*)g - i(\hat{Q}g^*).
\end{equation*}

The first two terms on each side cancel again, so we have (canceling the $i$'s):

\begin{equation*}
    f^*(\hat{Q}g) - g^*(\hat{Q}f) = (\hat{Q}f^*)g - (\hat{Q}g^*).
\end{equation*}

If we now add to this the result from the previous $h(x) = f(x) + g(x)$, then we get

\begin{equation}
    2f^*(\hat{Q}g) = 2(\hat{Q}f^*)g,
\end{equation}

or

\begin{equation*}
    \boxed{\braket{f|\hat{Q}|g} = \braket{f|\hat{Q}^{\dagger}|g}.}
\end{equation*}
