\section{(4.3)}

We are told that a particle of mass $m$ moves in the $x$-direction under some potential $U = bx$.

\begin{parts}
%a
\item The kinetic energy is simply the classical $T = \frac{1}{2}m\dot{x}^2$, and the potential is given, so our Lagrangian is:
\begin{equation}
    L = \frac{1}{2}m\dot{x}^2 - bx.
\end{equation}

%b
\item The first term in the Euler-Lagrange equation is
\begin{equation*}
    \diffp{L}{x} = -b,
\end{equation*}
and the second term is:
\begin{equation*}
    \diff{}{t}\diffp[]{L}{\dot{x}} = \diff{}{t}[m\dot{x}] = m\ddot{x}.
\end{equation*}
So, the full Euler-Lagrange equation is:
\begin{gather*}
    \diffp{L}{x} - \diff{}{t}\diffp[]{L}{\dot{x}} = -b - m\ddot{x} = 0, \\
    \rightarrow \boxed{m\ddot{x} + b = 0.}
\end{gather*}


%c
\item To solve, we first get just $\ddot{x}$ on one side:
\begin{equation*}
    \ddot{x} = -\frac{b}{m}.
\end{equation*}
Then we just integrate:
\begin{gather*}
    \dot{x} = -\frac{b}{m}\int \;\ddt = -\frac{b}{m}t + \dot{x}_0, \\
    x = \int \left(-\frac{b}{m}t + \dot{x}_0\right) \;\ddt = -\frac{b}{2m}t^2 + \dot{x}_0 t + x_0, \\
    \rightarrow \boxed{x(t) = -\frac{b}{2m}t^2 + \dot{x}_0 t + x_0.}
\end{gather*}



\end{parts}