\section{(4.12)}

The radial wavefunction is

\begin{equation}
    R_{n\ell} = \frac{1}{r}\rho^{\ell+1}e^{-\rho} v(\rho),
\end{equation}

where $\rho$ is an $n$th order polynominal whose coefficients are given by

\begin{equation}
    c_{j+1} = \frac{2(j+\ell+1-n)}{(j+1)(j+2\ell+2)}c_j,
\end{equation}

and $\rho = kr$ where $k=1/an = 1/3a$ for us with $n=3$.

Starting with $R_{30}$, let's start with computing the coefficients for the polynomial $v(\rho)$. Since we are told to not bother normalizing, I'll just set $c_0=1$ for simplicity. Therefore,

\begin{align}
    c_1 &= \frac{2(1-3)}{(1)(2)} = -2 \\
    c_2 &= (-2)\frac{2(1+1-3)}{(2)(3)} = \frac{-2}{6}(-2) = \frac{2}{3}, \\
    c_3 &= \br{\frac{2}{3}}\frac{2(2+1-3)}{\ldots} = 0,
\end{align}

where we don't care about the denominator in the last term since the numerator is zero. Therefore, our polynominal

\begin{equation}
    1 - 2\rho + \frac{2}{3}\rho^2 \rightarrow 1 - 2\frac{r}{3a} + \frac{2}{3}\br{\frac{r}{3a}}^2 = 1 - \frac{2}{3}\br{\frac{r}{a}} + \frac{2}{27}\br{\frac{r}{a}}^2.
\end{equation}

Thus,

\begin{align}
    R_{30} &= \frac{1}{r}\br{\frac{r}{3a}}e^{-r/3a}\left[ 1 - \frac{2}{3}\br{\frac{r}{a}} + \frac{2}{27}\br{\frac{r}{a}}^2 \right] \\
    \Aboxed{R_{30} &= \frac{1}{3a}e^{-r/3a}\left[ 1 - \frac{2}{3}\br{\frac{r}{a}} + \frac{2}{27}\br{\frac{r}{a}}^2 \right].}
\end{align}

Next, we consider $R_{31}$. The coefficients are, with $c_0=1$:

\begin{align}
    c_1 &= \frac{2(1+1-3)}{(1)(2+2)} = \frac{-1}{2}, \\
    c_2 &= \br{-\frac{1}{2}}\frac{2(1+1+1-3)}{\ldots} = 0,
\end{align}

where again we can stop before doing the denominator since the numerator is zero. Thus,

\begin{align}
    R_{31} &= \frac{1}{r}\br{\frac{r}{3a}}^2 e^{-r/3a} \left[ 1 - \frac{1}{2}\br{\frac{r}{3a}} \right] \\
    \Aboxed{R_{31} &= \frac{r}{9a^2}e^{-r/3a} \left[ 1 - \frac{1}{6}\br{\frac{r}{a}} \right].}
\end{align}

Lastly, for $R_{32}$, I'll take $c_0=1$ so

\begin{equation}
    c_1 = \frac{2(2+1-3)}{\ldots} = 0,
\end{equation}

so we only have the constant term. Thus,

\begin{gather}
    R_{32} = \frac{1}{r}\br{\frac{r}{3a}}^3 e^{-r/3a} \\
    \boxed{R_{32} = \frac{r^2}{27a^3}e^{-r/3a}.}
\end{gather}

