\section{(4.21)}

We are considering the raising and lowering operators for angular momentum, where

\begin{equation}
    L_+ f_{\ell}^m = A_{\ell}^m f_{\ell}^{m+1} \quad\mathrm{and}\quad L_- f_{\ell}^m = B_{\ell}^m f_{\ell}^{m-1},
\end{equation}

where $A_{\ell}^m$ and $B_{\ell}^m$ are undetermined functions of $\ell$ and $m$ and 

\begin{equation}
    L_{\pm} \equiv L_x \pm iL_y.
\end{equation}

First, we are to show that $L_+ = (L_-)^{\dagger}$ (and vice versa). This is straightforward:

\begin{equation}
    \braket{f | L_+ | g} = \int f^* [(L_x + iL_y)g] \;\ddx = \int [(L_x - iL_y)f]^* g \;\ddx = \Braket{f | (L_-)^{\dagger} | g},
\end{equation}

so, evidently, $L_+ = (L_-)^{\dagger}$.

Next, what we can do is use this fact so that

\begin{equation}
    \braket{f_{\ell}^m | L_-L_+ | f_{\ell}^m} = \Braket{f_{\ell}^m | (L_+)^{\dagger}L_+ | f_{\ell}^m} = \abs{A_{\ell}^m}^2 \braket{f_{\ell}^{m+1} | f_{\ell}^{m+1}} = \abs{A_{\ell}^m}^2.
\end{equation}

We can use Equation~(4.112) from the book to get that

\begin{equation}
    L_-L_+ = L^2 - L_z^2 - \hbar L_z
\end{equation}

so that

\begin{align}
    \abs{A_{\ell}^m}^2 &= \braket{f_{\ell}^m | L_-L_+ | f_{\ell}^m} = \Braket{f_{\ell}^m | L^2 - L_z^2 - \hbar L_z | f_{\ell}} \\
    &= [\hbar^2 \ell(\ell+1) - \hbar^2m^2 - \hbar^2m] \braket{f_{\ell}^m | f_{\ell}^m} \\
    \abs{A_{\ell}^m}^2 &= [\hbar^2 \ell(\ell+1) - \hbar^2m^2 - \hbar^2m].\label{eq:1}
\end{align}

So,

\begin{equation}
    \boxed{A_{\ell}^m = \hbar \sqrt{\ell(\ell+1) - m(m+1)}.}
\end{equation}

For the other case, we have

\begin{equation}
    \braket{f_{\ell}^m | L_+L_- | f_{\ell}^m} = \abs{B_{\ell}^m}^2,
\end{equation}

and the only difference between $L_-L_+$ (from before) and $L_+L_-$ (now) is a relative minus on the $\hbar L_z$ term in Equation~(4.112) in Griffiths. Therefore, we have a plus instead in the third term in brackets in Equation~\eqref{eq:1} (in this document) meaning

\begin{equation}
    \boxed{B_{\ell}^m = \hbar\sqrt{\ell(\ell+1) - m(m-1)}.}
\end{equation}

More succinctly, we could say

\begin{equation}
    L_{\pm}f_{\ell}^m = \hbar \sqrt{\ell(\ell+1) - m(m \pm 1)} f_{\ell}^{m \pm 1}.
\end{equation}