%2) Prove the relations for the gamma matrices in the attachment below. 
\section{}

\newcommand{\psl}{\slashed{p}}
\newcommand{\gsl}{\slashed{q}}

\begin{parts}
    \item First:
        \begin{align*}
            \psl\gsl + \gsl\psl &= \gamma^{\mu}p_{\mu}\gamma^{\nu}q_{\nu} + \gamma^{\nu}q_{\nu}\gamma^{\mu}p_{\mu} \\
            &= p_{\mu}q_{\nu}(\gamma^{\mu}\gamma^{\nu} + \gamma^{\mu}\gamma^{\nu}) \\
            &= 2g^{\mu\nu}p_{\mu}q_{\nu} = \boxed{2\dotprod{p}{q}}
        \end{align*}
    
    \item 
        \begin{align*}
            \gamma^{\mu}\gamma_{\mu} = \frac{1}{2}(\gamma^{\mu}\gamma_{\mu} + \gamma^{\nu}\gamma_{\nu}) = \frac{1}{2}g_{\mu\nu}(\gamma^{\mu}\gamma^{\nu} + \gamma^{\nu}\gamma^{\mu}) = g_{\mu\nu}g^{\mu\nu} = \boxed{4.}
        \end{align*}

    \item 
        \begin{align*}
            \gamma_{\mu}\gamma^{\nu}\gamma^{\mu} &= \gamma_{\mu}(\gamma^{\nu}\gamma^{\mu} + \gamma^{\mu}\gamma^{\nu} - \gamma^{\mu}\gamma^{\nu}), \\
            &= \gamma_{\mu}(2g^{\mu\nu} - \gamma^{\mu}\gamma^{\nu}) \\
            &= 2g^{\nu} - \gamma_{\mu}\gamma^{\mu}\gamma^{\nu} = 2\gamma^{\nu} - 4\gamma^{\nu} = \boxed{-2\gamma^{\nu}.}
        \end{align*}
        Since the components of the 4-momentum are just scalars, we can move them around however we want to easily say
        \begin{equation*}
            \gamma_{\mu}\psl\gamma^{\mu} = \gamma_{\mu}\gamma^{\nu}\gamma^{\mu}p_{\nu} = -2\gamma^{\nu}p_{\nu} = \boxed{-2\psl.}
        \end{equation*}
\end{parts}