\section{}

We are to show that the first component of the conjugate momentum for the free Lagrangian for a gauge field with the Feynman gauge fixing term given by 

\begin{equation}
    \lag = -\frac{1}{4}F_{\mu\nu}F^{\mu\nu} - \frac{1}{2}(\ddp_{\mu}A^{\mu})^2
\end{equation}

is

\begin{equation}
    \pi^0 = \pd{\lag}{\dot{A}_0} = -\ddp_{\mu}A^{\mu}.
\end{equation}

Firstly, it is easy to note that 

\begin{equation*}
    \pd{}{\dot{A}_0}{-\frac{1}{4}F_{\mu\nu}F^{\mu\nu}} = 0,
\end{equation*}

since the only components containing $\ddp_0A_0$ at all are the $F^{00}$ terms, which are zero. Turning to the other term, we have:

\begin{equation*}
    -\frac{1}{2}\br{\ddp_{\mu}A^{\mu}}^2 = -\frac{1}{2}\br{\ddp_0A^0  + \ddp_iA^i}^2 = -\frac{1}{2}\br{\dot{A}_0  + \ddp_iA^i}^2.
\end{equation*}

With this,

\begin{equation*}
    \pd{}{\dot{A}_0}{-\frac{1}{2}(\ddp_{\mu}A^{\mu})^2} = -\br{\dot{A}_0  + \ddp_i A^i} = -\ddp_{\mu}A^{\mu},
\end{equation*}

as expected.