\documentclass[titlepage]{article}
\usepackage{PreambleCommon,Preamble}


\title{HW5 \\[5pt] PHYS4210: Quantum Mechanics}
\author{Casey Hampson}

\begin{document}
    \maketitle
    \pagebreak

    \section{}

    The normalized spherical harmonics are given by

    \begin{equation}
      Y^m_\ell (\theta,\phi) = \sqrt{\frac{(2\ell + 1)}{4\pi} \frac{(\ell - m)!}{(\ell + m)!} } e^{im\phi} P^m_\ell (\cos\phi),
    \end{equation}

    where 

    \begin{equation}
      P^m_\ell (x) = (-1)^m (1-x^2)^{m/2} \br{\diff{}{x}}^m P_\ell (x),
    \end{equation}

    and

    \begin{equation}
      P_\ell (x) = \frac{1}{2^\ell l!} \br{\diff{}{x}}^\ell (x^2 - 1)^\ell.
    \end{equation}

    Starting with $m=\ell=0$, we can tell pretty easily that $P_0(\cos\theta) = 1$, and so too will $P^0_0(\cos\theta)$. Therefore,

    \begin{equation}
      \boxed{Y^0_0(\theta,\phi) = \sqrt{\frac{1}{4\pi}}.}
    \end{equation}

    For $\ell=1$ and $m=0$,

    \begin{align}
      P_1(x) &= \frac{1}{2}\diff{}{x}(x^2-1) = x \rightarrow \cos\theta, \\
      \rightarrow P^0_1 &= \cos\theta, \\
      \Aboxed{Y^0_1(\theta,\phi) &= \sqrt{\frac{3}{4\pi}}\cos\theta.}.
    \end{align}

    For $\ell=m=1$:

    \begin{align}
      P_1(x) &= x \rightarrow \cos\theta \\
      P^1_1(x) &= (-1) \sqrt{1-x^2} \diff{}{x}(x) = -\sqrt{1-x^2} \rightarrow -\sqrt{1 - \cos^2\theta} = -\sin\theta, \\
      \Aboxed{Y^1_1(\theta,\phi) &= - \sqrt{\frac{3}{8\pi}}e^{i\phi} \sin\theta.}
    \end{align}

    For $\ell=2$ and $m=0$:

    \begin{align}
      P_2(x) &= \frac{1}{8} \diff[2]{}{x}(x^2-1)^2 \\
             &= \frac{1}{8} \diff{}{x}[4x(x^2-1)] \\
             &= \frac{1}{8} [4(x^2-1) + 8x^2] \\
             &= \frac{1}{8} (12x^2 - 4) \\
             &\rightarrow \frac{1}{2}(\cos^2\theta - 1). \\
      P^0_2(\cos\theta) &= \frac{1}{2}(\cos^2\theta - 1). \\
      \Aboxed{Y^0_2(\theta,\phi) &= \sqrt{\frac{5}{16\pi}} (\cos^2\theta-1),}
    \end{align}

    where I brought the 1/2 from $P_2(x)$ inside the square root. For $\ell=2$ and $m=1$,

    \begin{align}
      P_2(x) &= \frac{1}{2}(3x^2 - 1) \rightarrow \frac{1}{2}(3\cos^2\theta - 1), \\
      P^1_2(x) &= - \sqrt{1 - x^2} \diff{}{x}\left[\frac{1}{2}(3x^2-1) \right] \\
             &\rightarrow -\sin\theta \cdot 3x \rightarrow -3\sin\theta\cos\theta, \\
      Y^1_2(\theta,\phi) &= -3 \sqrt{\frac{5}{4\pi} \frac{1}{3!}} e^{i\phi} \sin\theta\cos\theta, \\
      \Aboxed{Y^1_2(\theta,\phi) &= -\sqrt{\frac{15}{8\pi}} e^{i\phi}\sin\theta\cos\theta.}
    \end{align}

    Lastly, for $\ell=2$ and $m=-2$, we need to use the footnote 5 on page 135 for the definition of the associated Legendre functions for a negative $m$:

    \begin{align}
      P_2(x) &= \frac{1}{2} (3x^2 - 1) \rightarrow \frac{1}{2})c\cos^2\theta - 1) \\
      P^2_2(x) &= (-1)^2 (1-x^2) \diff[2]{}{x}\left[ \frac{1}{2}(3x^2 - 1) \right] \\
             &= 3x^2 \rightarrow 3\sin^2\theta, \\
      P^{-2}_2(x) &= (-1)^2 \frac{1}{4!} \cdot 3x^2 \rightarrow \frac{1}{8}\sin^2\theta, \\
      Y^{-2}_2(\theta,\phi) &= \frac{1}{8}\sqrt{\frac{5}{4\pi} \cdot 4!} e^{-2i\phi} \sin^2\theta \\
      \Aboxed{Y^{-2}_2(\theta,\phi) &= \sqrt{\frac{15}{32\pi}} e^{-2i\phi}\sin^2\theta.}      
    \end{align}

    



    \begin{figure}[ht]
      \centering
      \includegraphics[scale=0.8]{./res/Figs/fig_0_0.pdf}
      \caption{Spherical harmonic $Y^0_0(\theta,\phi)$}
      \label{fig:00}
    \end{figure}




    \begin{figure}[ht]
      \centering
      \includegraphics[scale=0.8]{./res/Figs/fig_0_1.pdf}
      \caption{Spherical harmonic $Y^0_1(\theta,\phi)$}
      \label{fig:01}
    \end{figure}

    


    \begin{figure}[ht]
      \centering
      \includegraphics[scale=0.8]{./res/Figs/fig_0_2.pdf}
      \caption{Spherical harmonic $Y^0_2(\theta,\phi)$}
      \label{fig:02}
    \end{figure}




    \begin{figure}[ht]
      \centering
      \includegraphics[scale=0.8]{./res/Figs/fig_1_1.pdf}
      \caption{Spherical harmonic $Y^1_1(\theta,\phi)$}
      \label{fig:11}
    \end{figure}




    \begin{figure}[ht]
      \centering
      \includegraphics[scale=0.8]{./res/Figs/fig_1_2.pdf}
      \caption{Spherical harmonic $Y^1_2(\theta,\phi)$}
      \label{fig:12}
    \end{figure}



    \begin{figure}[ht]
      \centering
      \includegraphics[scale=0.8]{./res/Figs/fig_-2_2.pdf}
      \caption{Spherical harmonic $Y^{-2}_2(\theta,\phi)$}
      \label{fig:-22}
    \end{figure}
    

    

    


\end{document}

%%% Local Variables:
%%% mode: LaTeX
%%% TeX-master: t
%%% End:


