%16.2

\section{(16.2)}


Let's just plug in:

\begin{align*}
    \left\{\gamma^0,\ \gamma^1\right\} &= \gamma^0\gamma^1 + \gamma^1\gamma^0, \\
    &= \begin{pmatrix}1 & 0 \\ 0 & -1\end{pmatrix}\begin{pmatrix}\sigma^1 & 0 \\ 0 & -\sigma^1\end{pmatrix} + \begin{pmatrix}\sigma^1 & 0 \\ 0 & -\sigma^1\end{pmatrix}\begin{pmatrix}1 & 0 \\ 0 & -1\end{pmatrix}, \\ 
    &= \begin{pmatrix}0 & \sigma^1 \\ \sigma^1 & 0\end{pmatrix} + \begin{pmatrix}0 & -\sigma^1 \\ -\sigma^1 & 0\end{pmatrix}, \\ 
    &= \begin{pmatrix}0 & 0 \\ 0 & 0\end{pmatrix} = 2g^{01} = 0,
\end{align*}

as expected.