\section{(2.22)}

\begin{parts}
    \item 
        \begin{equation*}
            \int_{-3}^1 (x^3 - 3x^2 + 2x - 1)\delta(x+2) \;\ddx = (-2)^3 - 3(-2)^2 + 2(-2) - 1 = -8-12-4-1 = \boxed{-25}.
        \end{equation*}
    \item 
        \begin{equation*}
            \int_0^{\infty} [\cos(3x) + 2]\delta(x - \pi) \;\ddx = \cos(3\pi) + 2 = -1 + 2 = \boxed{1}.
        \end{equation*}
    \item 
        \begin{equation*}
            \int_{-1}^1 e^{\abs{x} + 3} \delta(x-2) \;\ddx = 0,
        \end{equation*}
        since the delta function delivers its spike at $x=2$, which is outside the domain of the integral.
\end{parts}