\section{(2.26)}

The definition of the Fourier transform is

\begin{equation*}
    f(x) = \frac{1}{\sqrt{2\pi}}\intinf F(k) e^{ikx} \;\ddk,
\end{equation*}

and the inverse Fourier transform is

\begin{equation*}
    F(k) = \frac{1}{\sqrt{2\pi}}\intinf f(x) e^{-ikx} \;\ddx.
\end{equation*}

Here we have $f(x) \equiv \delta(x)$, so its Fourier transform is

\begin{equation*}
    F(k) = \frac{1}{\sqrt{2\pi}} \intinf \delta(x)e^{-ikx} \;\ddx = \frac{1}{\sqrt{2\pi}}.
\end{equation*}

Therefore

\begin{equation*}
    f(x) = \delta(x) = \frac{1}{\sqrt{2\pi}} \intinf \frac{1}{\sqrt{2\pi}} e^{ikx} \;\ddk = \frac{1}{2\pi} \intinf e^{ikx} \;\ddx.
\end{equation*}